transformations/Moore2MealyALT/MooreSemantics.v
@@ -8,14 +8,14 @@ Require Import core.utils.Utils.
 Require Import Id.
 
 Definition initialState (m: M) : option State_t :=
-    find_lift (get_E_data State_K) (fun s => NodeId_beq (Id "S0") s.(State_id)) m.(modelElements).
+    find_State (fun s => NodeId_beq (Id "S0") s.(State_id)) m.(modelElements).
 
 Definition State_outTransitions (m: M) (s: State_t) : list Transition_t :=
     filter_lift 
       (get_E_data Transition_K) 
       (fun t => 
          match (getTransition_source m t) with
-         | Some s' => State_t_beq s s'
+         | Some s' => State_t_beq s s' (* fixme : compare only the ids ? *)
          | None => false
          end)
       m.(Model.modelElements).
@@ -48,6 +48,45 @@ Definition execute (m: M) (input: list string) : option (list string) :=
     | Some s => executeFromState m s input
     | None => None
     end.
+
+
+(* get_Transition_target          getTransition_source *)
+(*                 \               /                   *)
+(*                  \             /                    *)
+(*                   \          State_outTransitions   *)
+(*                    \         /                      *)             
+(*                     \       /                       *)
+(*                      \    State_acceptTransition    *)
+(*                       \   /                         *)  
+(*                        \ /                          *)
+(*                       search                        *)
+(*                        /                            *)
+(*                       /                             *)
+(*     initialState    executeFromState                *)
+(*                 \   /                               *)
+(*                  \ /                                *)
+(*                execute                              *)
+
+
+(** Some tactics *)
+
+Lemma State_out_transitions_inv m s t :
+  List.In t (State_outTransitions m s) ->
+  List.In (TransitionElement t) (Model.modelElements m)
+  /\ getTransition_source m t = Some s.
+Proof.
+  intro H.
+  unfold State_outTransitions in H.
+  apply OptionListUtils.filter_lift_in in H.
+  destruct H as (? & ? & ? & ?).                   
+  PropUtils.destruct_match H1 ; [ | discriminate H1]. 
+  apply lem_State_t_beq_id in H1. subst s0.    
+  destruct x ;[discriminate H0 | PropUtils.inj H0]. (* monadInv *) 
+  auto.
+Qed.
+
+
+(** Some tests *)
 
 Require Import transformations.Moore2MealyALT.tests.sampleMoore.
 
