transformations/Moore2MealyALT/MooreWF.v
@@ -10,6 +10,7 @@ Definition unique_ids (m:Moore.M) :=
     e1.(State_id) = e2.(State_id) ->
     e1 = e2.
 
+(* fixme : move-me *)
 Lemma In_state : forall (m:Moore.M) e,
          List.In (StateElement e) (Model.modelElements m) <-> List.In e
     (OptionListUtils.lift_list (get_E_data State_K)
@@ -29,6 +30,7 @@ Proof.
   }
 Qed.
 
+(* fixme : move-me *)
 Lemma In_transition : forall (m:Moore.M) e,
          List.In (TransitionElement e) (Model.modelElements m) <-> List.In e
     (OptionListUtils.lift_list (get_E_data Transition_K)
@@ -53,7 +55,7 @@ Lemma discr  (m : M) :
   unique_ids m ->
   forall (i : NodeId),
     ListUtils.discriminating_predicate
-      (fun x : State_t => NodeId_beq i (State_id x) = true)
+      (fun x => NodeId_beq i (State_id x) = true)
       (OptionListUtils.lift_list (get_E_data State_K)
          (Model.modelElements m)).
 Proof.
@@ -72,8 +74,8 @@ Lemma in_find :
     unique_ids m ->
     List.In (StateElement e) m.(Model.modelElements) ->
     e.(State_id) = n ->
-    OptionListUtils.find_lift (get_E_data State_K)
-           (fun s : State_t => (NodeId_beq n  s.(State_id)))
+    find_State
+           (fun s => NodeId_beq n  s.(State_id))
            m.(Model.modelElements) = 
          Some e.
 Proof.
@@ -86,13 +88,15 @@ Qed.
 
 
 
-Lemma getTransition_source_some (s:State_t) t (m:Moore.M) :
+Lemma getTransition_source_some (m:Moore.M) :
   unique_ids m ->
-  List.In (StateElement s) m.(Model.modelElements) ->
-  State_id s = t.(Transition_source) ->
-  getTransition_source m t = Some s. 
+  forall s,
+    List.In (StateElement s) m.(Model.modelElements) ->
+    forall t,
+      State_id s = t.(Transition_source) ->
+      getTransition_source m t = Some s. 
 Proof.
-  intros WF H1 H2.
+  intros WF s H1 t H2.
   unfold getTransition_source.
   eapply OptionListUtils.in_find_lift ; [ | | | exact H1 ].
   { apply discr. assumption. }
@@ -100,13 +104,15 @@ Proof.
   { apply internal_NodeId_dec_lb. auto. }  
 Qed.
  
-Lemma getTransition_target_some (s:State_t) t (m:Moore.M) :
-  unique_ids m ->
-  List.In (StateElement s) m.(Model.modelElements) ->
-  State_id s = t.(Transition_dest) ->
-  getTransition_target m t = Some s. 
+Lemma getTransition_target_some (m:Moore.M) :
+  unique_ids m ->  
+  forall s, 
+    List.In (StateElement s) m.(Model.modelElements) ->
+    forall t,
+      State_id s = t.(Transition_dest) ->
+      getTransition_target m t = Some s. 
 Proof.
-  intros WF H1 H2.
+  intros WF s H1 t H2.
   unfold getTransition_target.
   eapply OptionListUtils.in_find_lift ; [ | | | exact H1 ].
   { apply discr. assumption. }
@@ -123,3 +129,38 @@ Definition determinist (m:Moore.M) :=
       t1.(Transition_source) = t2.(Transition_source) ->
       t1.(Transition_input) = t2.(Transition_input) ->
       t1 = t2.
+
+Lemma truc m :
+  determinist m ->
+  forall s i,
+    ListUtils.discriminating_predicate
+      (fun x : Transition_t =>
+         (i =? Transition_input x)%string = true)
+      (MooreSemantics.State_outTransitions m s).
+Proof.
+  intro WF.
+  intros s i.
+  intros t1 t2 H1 H2 P1 P2.
+  unfold State_outTransitions in H1, H2.
+  apply OptionListUtils.filter_lift_in in H1, H2.
+  destruct H1 as ( ? & ? & ? & ?).
+  destruct H2 as ( ? & ? & ? & ?).
+  PropUtils.destruct_match H1 ; [ | discriminate H1].
+  PropUtils.destruct_match H4 ; [ | discriminate H4].
+  destruct x ; [ discriminate H0 | PropUtils.inj H0]. (* monadInv *)
+  destruct x0 ; [ discriminate H3 | PropUtils.inj H3]. (* monadInv *)
+  apply internal_State_t_dec_bl in H1, H4.
+  subst s1 s0.
+  apply WF ; auto ; [ | ].
+  {
+    apply getTransition_source_inv in Heqo, Heqo0.
+    destruct Heqo.
+    destruct Heqo0.
+    congruence.
+  }
+  {
+    apply String.eqb_eq in P1.
+    apply String.eqb_eq in P2.
+    congruence.
+  }
+Qed.
