transformations/Moore2MealyALT/theorems/GettersCommut.v
@@ -1,0 +1,344 @@
+Require Moore2MealyALT.MooreSemantics.
+Require Moore2MealyALT.MealySemantics.
+Require Moore2MealyALT.Moore2Mealy.
+Require Moore2MealyALT.MooreWF.
+Require Moore2MealyALT.MealyWF.
+Require Moore2MealyALT.theorems.Elements.
+Require Moore2MealyALT.theorems.WFStable.
+
+Import String.
+
+Lemma getTransition_source_commut_fw m t :
+  Moore.WF_source m ->
+  forall s t',
+      Moore.getTransition_source m t = Some s ->
+      Elements.convert_transition m t = Some t' ->
+      Mealy.getTransition_source (Semantics.execute Moore2Mealy.Moore2Mealy m) t' = Some (Elements.convert s).
+Proof.
+  intros.
+  apply Moore.getTransition_source_inv in H0.
+  destruct H0.
+
+  apply MealyWF.getTransition_source_some.
+  { apply MealyWF.always_unique_ids. }
+  { apply Elements.state_element_fw. assumption. }
+  { 
+    apply Elements.convert_transition_inv in H1.
+    destruct H1 as (?&?&?) ; subst.
+    unfold Elements.convert.
+    simpl.
+    auto.
+  }
+Qed.
+
+Lemma getTransition_source_commut_none_fw m t :
+  Moore.WF_source m ->
+  forall  t',
+      Moore.getTransition_source m t = None ->
+      Elements.convert_transition m t = Some t' ->
+      Mealy.getTransition_source (Semantics.execute Moore2Mealy.Moore2Mealy m) t' = None.
+Proof.
+  intros.
+  unfold Moore.getTransition_source in H0.
+  unfold Mealy.getTransition_source.
+  unfold Elements.convert_transition in H1.
+  PropUtils.destruct_match H1 ; [ PropUtils.inj H1 | discriminate H1]. (* monadInv *)
+  unfold Mealy.Transition_source.
+  apply OptionListUtils.find_none.
+  intro e.
+  intro.
+
+  destruct e.
+  {
+    right.
+    destruct (Elements.state_element_bw _ _ H1).
+    destruct H2.
+    subst.
+    
+    eapply OptionListUtils.find_none in H0 ; eauto.  
+    destruct H0 ; [ discriminate | ].
+    destruct H0 as (?&?&?).
+    unfold Mealy.get_E_data.
+    eexists ; split ; [ reflexivity | ].
+    unfold Elements.convert. simpl.
+    unfold Moore.get_E_data in H0.
+    PropUtils.inj H0.
+    assumption.
+  }
+  { left. reflexivity. }
+Qed.
+
+Lemma getTransition_source_commut_bw m t :
+  Moore.WF_source m ->
+  forall s t',
+      Mealy.getTransition_source (Semantics.execute Moore2Mealy.Moore2Mealy m) t' = Some (Elements.convert s) ->
+      Elements.convert_transition m t = Some t' ->
+      exists s', s'.(Moore.State_id) = s.(Moore.State_id) /\ 
+      Moore.getTransition_source m t = Some s'. (* weak result because convert is not injective *)
+Proof.
+  intro WF ; intros.
+  destruct (Mealy.getTransition_source_inv _ _ _ H).
+  destruct (Elements.state_element_bw _ _ H1) as (?&?&?).
+  unfold Elements.convert in H4.
+  PropUtils.inj H4.
+
+  unfold Moore.getTransition_source.
+  rewrite OptionListUtils.find_lift_filter_lift.
+    unfold Elements.convert_transition in H0.
+  PropUtils.destruct_match H0 ; [ PropUtils.inj H0 | discriminate H0]. (* monadIv *)
+  simpl in H2.
+  
+  cut (exists s' : Moore.State_t,
+    List.find
+      (fun s0 : Moore.getTypeByEKind Moore.State_K =>
+       Id.NodeId_beq (Moore.Transition_source t) (Moore.State_id s0))
+      (OptionListUtils.lift_list (Moore.get_E_data Moore.State_K)
+         (Model.modelElements m)) = Some s').
+  { 
+    intros (s2&?). exists s2.
+    destruct (List.find_some _ _ H0).
+    split ; auto.
+    apply Id.internal_NodeId_dec_bl in H6.
+    rewrite <- H2.
+    rewrite <- H6.
+    reflexivity.
+  }
+  {
+    eapply ListUtils.find_some_left.
+    apply MooreWF.In_state. (*fixme : pas défini au bon endroit. *)
+    eassumption.
+    apply Id.internal_NodeId_dec_lb.
+    congruence.
+  }
+Qed.
+
+(* FIXME : this should be the main bw lemma *)
+Corollary getTransition_source_commut_bw_alt m t :
+  Moore.WF_source m ->
+  forall s' t',
+      Mealy.getTransition_source (Semantics.execute Moore2Mealy.Moore2Mealy m) t' = Some s' ->
+      Elements.convert_transition m t = Some t' ->
+      exists s, s' = Elements.convert s /\ 
+      Moore.getTransition_source m t = Some s. (* weak result because convert is not injective *)
+Proof.
+  intros.
+  replace s' with (Elements.convert (Moore.Build_State_t s'.(Mealy.State_id) ""%string)) in H0.
+  { 
+    eapply getTransition_source_commut_bw in H0 ; eauto.
+    destruct H0 as (?&?&?).
+    eexists ; split ; eauto.
+    unfold Elements.convert.
+    destruct x ; destruct s' ; simpl in * ; congruence.
+  }
+  { destruct s' ; reflexivity. }
+Qed.
+
+Corollary getTransition_source_commut_none_bw m t :
+  Moore.WF_source m ->
+  forall t',
+      Mealy.getTransition_source (Semantics.execute Moore2Mealy.Moore2Mealy m) t' = None ->
+      Elements.convert_transition m t = Some t' ->
+      Moore.getTransition_source m t = None. 
+Proof.
+  intros.
+  destruct (Moore.getTransition_source m t) eqn:? ; [ exfalso | reflexivity].
+  eapply getTransition_source_commut_fw in Heqo ; eauto.
+  congruence.
+Qed.
+ 
+Corollary getTransition_source_commut_none_fw_alt m t :
+  Moore.WF_source m ->
+  forall  t',
+      Moore.getTransition_source m t = None ->
+      Elements.convert_transition m t = Some t' ->
+      Mealy.getTransition_source (Semantics.execute Moore2Mealy.Moore2Mealy m) t' = None.
+Proof.
+  intros.
+  destruct (Mealy.getTransition_source
+    (Semantics.execute Moore2Mealy.Moore2Mealy m) t') eqn:?; [ exfalso | reflexivity ].
+  replace s with (Elements.convert (Moore.Build_State_t s.(Mealy.State_id) " "%string)) in Heqo.
+
+  eapply getTransition_source_commut_bw in Heqo ; eauto.
+  destruct Heqo as (?&?&?).
+  congruence.
+  destruct s ; reflexivity.
+Qed.
+
+(** [getTransition_target] : copy/paste [getTransition_source] *)
+
+
+Lemma getTransition_target_commut_fw m t :
+  Moore.WF_target m ->
+  forall s t',
+      Moore.getTransition_target m t = Some s ->
+      Elements.convert_transition m t = Some t' ->
+      Mealy.getTransition_target (Semantics.execute Moore2Mealy.Moore2Mealy m) t' = Some (Elements.convert s).
+Proof.
+  intros.
+  apply Moore.getTransition_target_inv in H0.
+  destruct H0.
+
+  apply MealyWF.getTransition_target_some.
+  { apply MealyWF.always_unique_ids. }
+  { apply Elements.state_element_fw. assumption. }
+  { 
+    apply Elements.convert_transition_inv in H1.
+    destruct H1 as (?&?&?) ; subst.
+    unfold Elements.convert.
+    simpl.
+    auto.
+  }
+Qed.
+
+Lemma getTransition_target_commut_none_fw m t :
+  Moore.WF_target m ->
+  forall  t',
+      Moore.getTransition_target m t = None ->
+      Elements.convert_transition m t = Some t' ->
+      Mealy.getTransition_target (Semantics.execute Moore2Mealy.Moore2Mealy m) t' = None.
+Proof.
+  intros.
+  unfold Moore.getTransition_target in H0.
+  unfold Mealy.getTransition_target.
+  unfold Elements.convert_transition in H1.
+  PropUtils.destruct_match H1 ; [ PropUtils.inj H1 | discriminate H1]. (* monadInv *)
+  unfold Mealy.Transition_dest.
+  apply OptionListUtils.find_none.
+  intro e.
+  intro.
+
+  destruct e.
+  {
+    right.
+    destruct (Elements.state_element_bw _ _ H1).
+    destruct H2.
+    subst.
+    
+    eapply OptionListUtils.find_none in H0 ; eauto.  
+    destruct H0 ; [ discriminate | ].
+    destruct H0 as (?&?&?).
+    unfold Mealy.get_E_data.
+    eexists ; split ; [ reflexivity | ].
+    unfold Elements.convert. simpl.
+    unfold Moore.get_E_data in H0.
+    PropUtils.inj H0.
+    assumption.
+  }
+  { left. reflexivity. }
+Qed.
+
+Lemma getTransition_target_commut_bw m t :
+  Moore.WF_target m ->
+  forall s t',
+      Mealy.getTransition_target (Semantics.execute Moore2Mealy.Moore2Mealy m) t' = Some (Elements.convert s) ->
+      Elements.convert_transition m t = Some t' ->
+      exists s', s'.(Moore.State_id) = s.(Moore.State_id) /\ 
+      Moore.getTransition_target m t = Some s'. (* weak result because convert is not injective *)
+Proof.
+  intro WF ; intros.
+  destruct (Mealy.getTransition_target_inv _ _ _ H).
+  destruct (Elements.state_element_bw _ _ H1) as (?&?&?).
+  unfold Elements.convert in H4.
+  PropUtils.inj H4.
+
+  unfold Moore.getTransition_target.
+  rewrite OptionListUtils.find_lift_filter_lift.
+    unfold Elements.convert_transition in H0.
+  PropUtils.destruct_match H0 ; [ PropUtils.inj H0 | discriminate H0]. (* monadIv *)
+  simpl in H2.
+  
+  cut (exists s' : Moore.State_t,
+    List.find
+      (fun s0 : Moore.getTypeByEKind Moore.State_K =>
+       Id.NodeId_beq (Moore.Transition_dest t) (Moore.State_id s0))
+      (OptionListUtils.lift_list (Moore.get_E_data Moore.State_K)
+         (Model.modelElements m)) = Some s').
+  { 
+    intros (s2&?). exists s2.
+    destruct (List.find_some _ _ H0).
+    split ; auto.
+    apply Id.internal_NodeId_dec_bl in H6.
+    rewrite <- H2.
+    rewrite <- H6.
+    reflexivity.
+  }
+  {
+    eapply ListUtils.find_some_left.
+    apply MooreWF.In_state. (*fixme : pas défini au bon endroit. *)
+    eassumption.
+    apply Id.internal_NodeId_dec_lb.
+    congruence.
+  }
+Qed.
+
+(* FIXME : this should be the main bw lemma *)
+Corollary getTransition_target_commut_bw_alt m t :
+  Moore.WF_target m ->
+  forall s' t',
+      Mealy.getTransition_target (Semantics.execute Moore2Mealy.Moore2Mealy m) t' = Some s' ->
+      Elements.convert_transition m t = Some t' ->
+      exists s, s' = Elements.convert s /\ 
+      Moore.getTransition_target m t = Some s. (* weak result because convert is not injective *)
+Proof.
+  intros.
+  replace s' with (Elements.convert (Moore.Build_State_t s'.(Mealy.State_id) ""%string)) in H0.
+  { 
+    eapply getTransition_target_commut_bw in H0 ; eauto.
+    destruct H0 as (?&?&?).
+    eexists ; split ; eauto.
+    unfold Elements.convert.
+    destruct x ; destruct s' ; simpl in * ; congruence.
+  }
+  { destruct s' ; reflexivity. }
+Qed.
+
+Lemma getTransition_target_commut_bw_alt_alt m :
+  Moore.WF_target m ->
+  forall s' t',
+    List.In (Mealy.TransitionElement t') (Semantics.execute Moore2Mealy.Moore2Mealy m).(Model.modelElements) ->  
+      Mealy.getTransition_target (Semantics.execute Moore2Mealy.Moore2Mealy m) t' = Some s' ->
+      exists t,
+      Elements.convert_transition m t = Some t' /\
+      exists s, s' = Elements.convert s /\ 
+      Moore.getTransition_target m t = Some s. (* weak result because convert is not injective *)
+Proof.
+  intros WF ; intros s' t' T_IN1 T_G. 
+  destruct (Mealy.getTransition_target_inv _ _ _ T_G) as (T_IN2 & T_E).
+
+  apply Elements.transition_element_bw in T_IN1 ; eauto.
+  destruct T_IN1 as (t & IN1 & T).
+  exists t.
+  split ; [ congruence | ].
+  eapply getTransition_target_commut_bw_alt ; eauto.
+Qed.
+
+Corollary getTransition_target_commut_none_bw m t :
+  Moore.WF_target m ->
+  forall t',
+      Mealy.getTransition_target (Semantics.execute Moore2Mealy.Moore2Mealy m) t' = None ->
+      Elements.convert_transition m t = Some t' ->
+      Moore.getTransition_target m t = None. 
+Proof.
+  intros.
+  destruct (Moore.getTransition_target m t) eqn:? ; [ exfalso | reflexivity].
+  eapply getTransition_target_commut_fw in Heqo ; eauto.
+  congruence.
+Qed.
+ 
+Corollary getTransition_target_commut_none_fw_alt m t :
+  Moore.WF_target m ->
+  forall  t',
+      Moore.getTransition_target m t = None ->
+      Elements.convert_transition m t = Some t' ->
+      Mealy.getTransition_target (Semantics.execute Moore2Mealy.Moore2Mealy m) t' = None.
+Proof.
+  intros.
+  destruct (Mealy.getTransition_target
+    (Semantics.execute Moore2Mealy.Moore2Mealy m) t') eqn:?; [ exfalso | reflexivity ].
+  replace s with (Elements.convert (Moore.Build_State_t s.(Mealy.State_id) " "%string)) in Heqo.
+
+  eapply getTransition_target_commut_bw in Heqo ; eauto.
+  destruct Heqo as (?&?&?).
+  congruence.
+  destruct s ; reflexivity.
+Qed.
